generic/Zeta.Generic.Blum.fsti
@@ -14,6 +14,17 @@ module S = FStar.Seq
 module SA = Zeta.SeqAux
 module G = Zeta.Generic.Global
 
+(* is this a blum add within epoch ep *)
+let is_blum_add_epoch (#vspec #n:_) (ep: epoch) (il: verifiable_log vspec n) (i: seq_index il)
+  = is_blum_add il i &&
+    (let be = blum_add_elem il i in
+     be.t.e = ep)
+
+let is_blum_evict_epoch (#vspec #n:_) (ep: epoch) (il: verifiable_log vspec n) (i: seq_index il)
+  = is_blum_evict il i &&
+    (let be = blum_evict_elem il i in
+     be.t.e = ep)
+
 val add_il (#vspec #n:_) (ep: epoch) (il: verifiable_log vspec n)
   : interleaving (ms_hashfn_dom vspec.app) n
 
@@ -25,6 +36,15 @@ let add_set #vspec #n (ep: epoch) (il: verifiable_log vspec n)
   : mset_ms_hashfn_dom vspec.app
   = seq2mset (add_seq ep il)
 
+val add_set_snoc (#vspec #n:_) (ep: epoch) (il: verifiable_log vspec n {length il > 0})
+  : Lemma (ensures (let i = length il - 1 in
+                    let il' = prefix il i in
+                    let as = add_set ep il in
+                    let as' = add_set ep il' in
+                    if is_blum_add_epoch ep il i then
+                      as == add_elem as' (blum_add_elem il i)
+                    else as == as'))
+
 val evict_il (#vspec #n:_) (ep: epoch) (il: verifiable_log vspec n)
   : interleaving (ms_hashfn_dom vspec.app) n
 
@@ -35,6 +55,15 @@ let evict_seq (#vspec #n:_) (ep: epoch) (il: verifiable_log vspec n)
 let evict_set #vspec #n (ep: epoch) (il: verifiable_log vspec n)
   : mset_ms_hashfn_dom vspec.app
   = seq2mset (evict_seq ep il)
+
+val evict_set_snoc (#vspec #n:_) (ep: epoch) (il: verifiable_log vspec n {length il > 0})
+  : Lemma (ensures (let i = length il - 1 in
+                    let il' = prefix il i in
+                    let as = evict_set ep il in
+                    let as' = evict_set ep il' in
+                    if is_blum_evict_epoch ep il i then
+                      as == add_elem as' (blum_evict_elem il i)
+                    else as == as'))
 
 let aems_equal_upto #vspec #n (epmax: epoch) (il: verifiable_log vspec n)
   = forall (ep: epoch). ep <= epmax ==> add_set ep il == evict_set ep il
